\question{
        Write out the terms of the expression
        and then evaluate.
    }
\begin{parts}
    \part{
        $$\sum_{j=-1}^2{\left((3j)^2-5j\right)}$$
    }
    \begin{solution}
        \begin{align*}
            \sum_{j=-1}^2{\left((3j)^2-5j\right)} &=
            \left((-3)^2+5\right) +
            \left((0)^2+0\right) +
            \left((3)^2-5\right) +
            \left((3*2)^2-5*2\right)\\
            & = 14+0+4+26 = 44
        \end{align*}
    \end{solution}

    \part{
        $$\prod_{k=2}^7{\left(1-\frac{1}{k^2}\right)}$$
    }
    \begin{solution}
        \begin{align*}
            \prod_{k=2}^7{\left(1-\frac{1}{k^2}\right)} &=
            \left(1-1/2^2\right)\cdot
            \left(1-1/3^2\right)\cdot
            \left(1-1/4^2\right)\cdot
            \left(1-1/5^2\right)\cdot
            \left(1-1/6^2\right)\cdot
            \left(1-1/7^2\right)\\
            & = \frac{3}{4} \cdot
            \frac{8}{9} \cdot
            \frac{15}{16} \cdot
            \frac{24}{25} \cdot
            \frac{35}{36} \cdot
            \frac{48}{49}=\frac{16}{21}\\
        \end{align*}
    \end{solution}
\end{parts}